playing with layered effects, dm4a

examples/layeredeffects/ND.fst
@@ -11,21 +11,20 @@ module F = FStar.FunctionalExtensionality
 module W = FStar.WellFounded
 module T = FStar.Tactics
 
-// m is a monad
+// m is a monad. In this particular example, lists
 val m (a : Type u#a) : Type u#a
 let m a = list a
 
-val m_return (a : Type) : a -> m a
-let m_return a x = [x]
+val m_return (#a : Type) : a -> m a
+let m_return x = [x]
 
-val m_bind (a : Type) (b : Type) : m a -> (a -> m b) -> m b
-let m_bind _ _ =
-  fun l f -> concatMap f l
+val m_bind (#a #b : Type) : m a -> (a -> m b) -> m b
+let m_bind l f = concatMap f l
 
 // w is an ordered (w_ord) monad with conjunction (w_conj) and actions from prop (w_act_prop)
+// In this example, good ol' continuations into prop
 val w0 (a : Type u#a) : Type u#(max 1 a)
 let w0 a = (a -> Type0) -> Type0
-
 
 let monotonic (w:w0 'a) =
   forall p1 p2. (forall x. p1 x ==> p2 x) ==> w p1 ==> w p2
@@ -33,34 +32,32 @@ let monotonic (w:w0 'a) =
 val w (a : Type u#a) : Type u#(max 1 a)
 let w a = w:(w0 a){monotonic w}
 
+val w_ord (#a : Type) : w a -> w a -> Type0
+let w_ord wp1 wp2 = forall p. wp1 p ==> wp2 p
 
-val w_ord (a : Type) : w a -> w a -> Type0
-let w_ord a wp1 wp2 = forall p. wp1 p ==> wp2 p
-
-val w_ord_trans (a : Type) (wp1 : w a) (wp2 : w a) (wp3 : w a) : Lemma (requires w_ord a wp1 wp2 /\ w_ord a wp2 wp3) (ensures w_ord a wp1 wp3)
-let w_ord_trans = fun _ _ _ _ -> ()
+val w_ord_trans (#a : Type) (wp1 : w a) (wp2 : w a) (wp3 : w a) : Lemma (requires w_ord wp1 wp2 /\ w_ord wp2 wp3) (ensures w_ord wp1 wp3)
+let w_ord_trans = fun _ _ _ -> ()
 
 // GM: this is "assume"
-val w_act_prop (a : Type) : Type0 -> w a -> w a
-let w_act_prop a phi wp = fun p -> phi ==> wp p
+val w_act_prop (#a : Type) : Type0 -> w a -> w a
+let w_act_prop phi wp = fun p -> phi ==> wp p
 
+val w_conj (#a : Type) : w a -> w a -> w a
+let w_conj wp1 wp2 p = wp1 p /\ wp2 p
 
-val w_conj (a : Type) : w a -> w a -> w a
-let w_conj a wp1 wp2 p = wp1 p /\ wp2 p
+val w_return (#a : Type) : a -> w a
+let w_return x = fun p -> p x
 
-val w_return (a : Type) : a -> w a
-let w_return a x = fun p -> p x
-
-val w_bind (a : Type) (b : Type) : w a -> (a -> w b) -> w b
-let w_bind a b wp1 k =
+val w_bind (#a #b : Type) : w a -> (a -> w b) -> w b
+let w_bind wp1 k =
   fun p -> wp1 (fun x -> k x p)
 
-val w_bind_monotonic (a : Type) (b : Type) (m1 : w a) (m2 : w a) (f1 : a -> w b) (f2 : a -> w b) : Lemma (requires w_ord a m1 m2 /\ (forall (a : a).{:pattern f2 a} w_ord b (f1 a) (f2 a))) (ensures w_ord b (w_bind a b m1 f1) (w_bind a b m2 f2))
-let w_bind_monotonic a b m1 m2 f1 f2 = ()
+val w_bind_monotonic (#a #b : Type) (m1 : w a) (m2 : w a) (f1 : a -> w b) (f2 : a -> w b) : Lemma (requires w_ord m1 m2 /\ (forall (a : a).{:pattern f2 a} w_ord (f1 a) (f2 a))) (ensures w_ord (w_bind m1 f1) (w_bind m2 f2))
+let w_bind_monotonic m1 m2 f1 f2 = ()
 
 // we can define an "equality" on w a
-val w_equiv (a : Type) : w a -> w a -> Type0
-let w_equiv a wp1 wp2 = w_ord a wp1 wp2 /\ w_ord a wp2 wp1
+val w_equiv (#a : Type) : w a -> w a -> Type0
+let w_equiv wp1 wp2 = w_ord wp1 wp2 /\ w_ord wp2 wp1
 
 // the monad morphism that connect the two monadic structures
 val interp (#a : Type) : m a -> w a
@@ -68,7 +65,7 @@ val interp (#a : Type) : m a -> w a
 let interp #a (l:list a) =
   fun p -> forall x. memP x l ==> p x
 
-val interp_ret (a : Type) (x : a) : Lemma (interp (m_return a x) `w_equiv a` w_return a x)
+val interp_ret (a : Type) (x : a) : Lemma (interp (m_return x) `w_equiv` w_return x)
 let interp_ret a x = ()
 
 
@@ -91,9 +88,9 @@ let rec concatmaplemma #a #b l f x =
     concatmaplemma t f x
 
 
-let dro_w a wp2 wp1 = w_ord a wp1 wp2
+let dro_w wp2 wp1 = w_ord wp1 wp2
 
-val interp_bind (a b : Type) (v : m a) (f : a -> m b) : Lemma (interp (m_bind a b v f) `w_equiv _` w_bind a b (interp v) (fun a -> interp (f a)))
+val interp_bind (a b : Type) (v : m a) (f : a -> m b) : Lemma (interp (m_bind v f) `w_equiv` w_bind (interp v) (fun a -> interp (f a)))
 
 // uses pattern above, slightly brittle too
 #push-options "--retry 10"
@@ -122,32 +119,28 @@ let interp_bind a b v f = ()
 // In layered effects, we instead construct the Dijkstra monad as a
 // sigma type (see the paper)
 
-let dm (a : Type) (wp : w a) : Type = v:m a{w_ord a wp (interp v)}
+let dm (a : Type) (wp : w a) : Type = v:m a{w_ord wp (interp v)}
 
-let irepr (a : Type) (wp: w a) = unit -> dm a wp
-let ireturn (a : Type) (x : a) : irepr a (w_return a x) = fun () -> interp_ret a x ; m_return a x
+let irepr (a : Type) (wp: w a) = dm a wp
+let ireturn (a : Type) (x : a) : irepr a (w_return x) = interp_ret a x ; m_return x
 
-let ibind (a : Type) (b : Type) (wp_v : w a) (wp_f: a ^-> w b) (v : irepr a wp_v) (f : (x:a -> irepr b (wp_f x))) : irepr b (w_bind a b wp_v wp_f) =
-  fun () ->
-  interp_bind a b (v ()) (fun x -> f x ()) ;
-  w_bind_monotonic a b wp_v (interp (v ())) wp_f (fun a -> interp (f a ()));
-  w_ord_trans b (w_bind a b wp_v wp_f) (w_bind a b (interp (v ())) (fun a -> interp (f a ()))) (interp (m_bind a b (v ()) (fun x -> f x ())));
-  m_bind a b (v ()) (fun x -> f x ())
- 
-let isubcomp (a:Type) (wp1 wp2: w a) (f : irepr a wp1) : Pure (irepr a wp2) (requires w_ord a wp2 wp1) (ensures fun _ -> True) =
-  fun () -> w_ord_trans a wp2 wp1 (interp (f ())) ; f () 
+let ibind (a : Type) (b : Type) (wp_v : w a) (wp_f: a -> w b) (v : irepr a wp_v) (f : (x:a -> irepr b (wp_f x))) : irepr b (w_bind wp_v wp_f) =
+  interp_bind a b v f;
+  m_bind v f
 
-let wp_if_then_else (a:Type) (wp1 wp2:w a) (p:Type0) : w a=
-  w_conj a (w_act_prop a p wp1) (w_act_prop a (~p) wp2)
+let isubcomp (a:Type) (wp1 wp2: w a) (f : irepr a wp1) : Pure (irepr a wp2) (requires w_ord wp2 wp1) (ensures fun _ -> True) = f
+
+let wp_if_then_else (#a:Type) (wp1 wp2:w a) (p:Type0) : w a=
+  w_conj (w_act_prop p wp1) (w_act_prop (~p) wp2)
 
 let i_if_then_else (a : Type) (wp1 wp2 : w a) (f : irepr a wp1) (g : irepr a wp2) (p : Type0) : Type =
-  irepr a (wp_if_then_else a wp1 wp2 p)
+  irepr a (wp_if_then_else wp1 wp2 p)
 
 let lem_if_1 (a:Type) (wp1 wp2 : w a) (p:Type0) (f : irepr a wp1) (g : irepr a wp2)
-  : Lemma (p ==> w_ord a (wp_if_then_else a wp1 wp2 p) wp1)
+  : Lemma (p ==> w_ord (wp_if_then_else wp1 wp2 p) wp1)
           [SMTPat ()]
   = 
-  let aux post : Lemma (requires p /\ wp_if_then_else a wp1 wp2 p post)
+  let aux post : Lemma (requires p /\ wp_if_then_else wp1 wp2 p post)
                        (ensures wp1 post)
     =
     calc (<==>) {
@@ -157,20 +150,20 @@ let lem_if_1 (a:Type) (wp1 wp2 : w a) (p:Type0) (f : irepr a wp1) (g : irepr a w
       <==> {}
       (p ==> wp1 post) /\ ((~p) ==> wp2 post);
       <==> {}
-      (w_act_prop a p wp1 post) /\ (w_act_prop a (~p) wp2 post);
+      (w_act_prop p wp1 post) /\ (w_act_prop (~p) wp2 post);
       <==> { _ by (compute ()) } // GM: why???
-      w_conj a (w_act_prop a p wp1) (w_act_prop a (~p) wp2) post;
-      <==> {}
-      wp_if_then_else a wp1 wp2 p post;
+      w_conj (w_act_prop p wp1) (w_act_prop (~p) wp2) post;
+      <==> { }
+      wp_if_then_else wp1 wp2 p post;
     }
   in
   Classical.forall_intro (Classical.move_requires aux)
   
 let lem_if_2 (a:Type) (wp1 wp2 : w a) (p:Type0) (f : irepr a wp1) (g : irepr a wp2)
-  : Lemma ((~p) ==> w_ord a (wp_if_then_else a wp1 wp2 p) wp2)
+  : Lemma ((~p) ==> w_ord (wp_if_then_else wp1 wp2 p) wp2)
           [SMTPat ()]
   = 
-  let aux post : Lemma (requires (~p) /\ wp_if_then_else a wp1 wp2 p post)
+  let aux post : Lemma (requires (~p) /\ wp_if_then_else wp1 wp2 p post)
                        (ensures wp2 post)
     =
     calc (<==>) {
@@ -180,11 +173,11 @@ let lem_if_2 (a:Type) (wp1 wp2 : w a) (p:Type0) (f : irepr a wp1) (g : irepr a w
       <==> {}
       (p ==> wp1 post) /\ ((~p) ==> wp2 post);
       <==> {}
-      (w_act_prop a p wp1 post) /\ (w_act_prop a (~p) wp2 post);
+      (w_act_prop p wp1 post) /\ (w_act_prop (~p) wp2 post);
       <==> { _ by (compute ()) } // GM: why???
-      w_conj a (w_act_prop a p wp1) (w_act_prop a (~p) wp2) post;
+      w_conj (w_act_prop p wp1) (w_act_prop (~p) wp2) post;
       <==> {}
-      wp_if_then_else a wp1 wp2 p post;
+      wp_if_then_else wp1 wp2 p post;
     }
   in
   Classical.forall_intro (Classical.move_requires aux)
@@ -203,41 +196,32 @@ layered_effect {
        if_then_else = i_if_then_else
 }
 
-assume Mono : forall (a:Type) (wp:pure_wp a). monotonic wp
-
-assume Pure_wp_corr : forall (a:Type) (wp:pure_wp a) (f:(unit -> PURE a wp))
-                        (p:pure_post a). wp p ==> p (f ())
-
-let lemgg (a:Type) (wp:pure_wp a) p q (_ : squash p) (_ : monotonic wp) :
-    Lemma (requires (wp (fun _ -> p)))
-          (ensures (wp (fun x -> q x ==> p))) = ()
-
-let lemhh (a:Type) (wp:pure_wp a) p (_ : squash p) :
-    Lemma (requires (wp (fun _ -> True)))
-          (ensures (wp (fun _ -> p))) = ()
-
-let lift_pure_nd (a:Type) (wp:pure_wp a) (f:(unit -> PURE a wp)) :
-  Pure (irepr a wp) (requires (wp (fun _ -> True)))
+let lift_pure_nd (a:Type) (wp:pure_wp a{monotonic wp}) (f:(unit -> PURE a wp)) :
+  Pure (irepr a wp) (requires (wp (fun _ -> True))) // <--- This is a lift from Tot only
                     (ensures (fun _ -> True))
-  = fun () -> admit (); [f ()] // GM : not sure why this fails
+  = [f ()]
 
 sub_effect PURE ~> ND = lift_pure_nd
 
+val test_f : unit -> ND int (fun p -> p 5 /\ p 3)
+let test_f () =
+  ND?.reflect [3; 5]
 
-assume val test_f : unit -> ND int (fun p -> p 5 /\ p 3)
+//let l () : (l:(list int){forall p. p 5 /\ p 3 ==> interp l p}) = reify (test_f ())
+// ^ This one doesn't work... datatype subtyping to blame?
 
-let l : unit -> (l:list int{forall p. p 5 /\ p 3 ==> interp l p}) = reify (test_f ())
+let l () : (l:(list int)) = reify (test_f ())
 
 effect Nd (a:Type) (pre:pure_pre) (post:pure_post' a pre) =
         ND a (fun (p:pure_post a) -> pre /\ (forall (pure_result:a). post pure_result ==> p pure_result))
 
 val choose : #a:Type0 -> x:a -> y:a -> ND a (fun p -> p x /\ p y)
 let choose #a x y =
-    ND?.reflect (fun () -> [x;y])
+    ND?.reflect [x;y]
 
 val fail : #a:Type0 -> unit -> ND a (fun p -> True)
 let fail #a () =
-    ND?.reflect (fun () -> [])
+    ND?.reflect []
 
 let flip () : ND bool (fun p -> p true /\ p false) =
     choose true false
@@ -287,4 +271,9 @@ let (pyths_norm : unit -> (Prims.int * Prims.int * Prims.int) Prims.list) =
     ((Prims.parse_int "6"), (Prims.parse_int "8"), (Prims.parse_int "10"));
     ((Prims.parse_int "8"), (Prims.parse_int "6"), (Prims.parse_int "10"))]
 *)
-let pyths_norm () = normalize_term (reify (pyths ()) ())
+let pyths_norm () = normalize_term (reify (pyths ()))
+
+(* ^ Try it in emacs: C-c C-s C-e pyths_norm ():
+Reducing ‘pyths_norm ()’…
+pyths_norm () ↓βδιζr [3, 4, 5; 4, 3, 5; 6, 8, 10; 8, 6, 10] <: list ((int * int) * int)
+*)
